First working version of new word-bitwise

model/isabelle/BW2.thy
@@ -1,23 +1,8 @@
 theory BW2
 
-imports "HOL-Word.Word_Bitwise"
+imports "Carry_Val"
 
 begin
-
-text \<open>
-Facts about the "carry" value. The carry object for x and y
-is, at every bit position, the value that would have been
-carried in during an addition of x and y. This can be used
-to rewrite additions and inequalities to factor out the
-components that move between bit positions.
-\<close>
-
-definition
-  carry_val :: "('a :: {bit_operations, plus, zero, one}) \<Rightarrow> 'a \<Rightarrow> bool \<Rightarrow> 'a"
-  where
-  "carry_val x y c = (x + y + (if c then 1 else 0)) XOR (x XOR y)"
-
-(* easy enough to define, no idea how to prove anything about it *)
 
 text \<open>
 Upgrade of the existing Word_Bitwise conversion to booleans.
@@ -31,248 +16,21 @@ fresh meta-bound variables. The latter form seems to be quite
 compatible with the Argo solver.
 \<close>
 
-lemma rbl_word_if_let: "rev (to_bl (if P then x else y)) =
-    (let c = P in map2 (If c) (rev (to_bl x)) (rev (to_bl y)))"
-  by (simp add: Product_Type.split_def)
-
-fun carry_chain :: "(bool * bool) list \<Rightarrow> bool \<Rightarrow> bool list"
-  where
-    "carry_chain [] x = []"
-  | "carry_chain (x # xs) y = y # carry_chain xs (carry (fst x) (snd x) y)"
-
-lemma length_carry_chain[simp]:
-  "length (carry_chain xs c) = length xs"
-  by (induct xs arbitrary: c, simp_all)
-
-lemma carry_chain_eq_Nil[simp]:
-  "(carry_chain xs c = []) = (xs = [])"
-  by (cases xs, simp_all)
-
-definition carry_word :: "('a :: len) word \<Rightarrow> 'a word \<Rightarrow> bool \<Rightarrow> 'a word"
-  where
-  "carry_word x y c = of_bl (rev (carry_chain (zip (rev (to_bl x)) (rev (to_bl y))) c))"
-
-lemma rbl_plus_carry_chain:
-  "length xs = length ys \<Longrightarrow>
-    rbl_plus c xs ys = map (\<lambda>(c, (x, y)). xor3 x y c)
-        (zip (carry_chain (zip xs ys) c) (zip xs ys))"
-  by (induct arbitrary: c rule: list_induct2, simp_all add: rbl_plus_simps)
-
-lemma carry_word_eq_xor:
-  "carry_word x y False = ((x + y) XOR x XOR y)"
-  apply (simp only: word_eq_rbl_eq Let_def rbl_word_plus rbl_word_xor)
-  apply (simp add: rbl_plus_carry_chain carry_word_def)
-  apply (rule nth_equalityI, simp_all)
-  apply (simp add: nth_rev xor3_def word_bl.Abs_inverse)
-  apply blast
-  done
-
-(* the silly cw AND cw part is to stop the let_alt simproc removing the let-binding *)
-lemma word_plus_carry_chain:
-  fixes x :: "('a :: len) word"
-  shows "x + y = (let xnm = x; ynm = y; cw = carry_word xnm ynm False in (xnm XOR ynm) XOR (cw AND cw))"
-  apply (simp add: Let_def carry_word_eq_xor)
-  apply (simp add: word_eq_iff word_ops_nth_size word_size)
-  apply blast
-  done
-
-lemmas word_minus_carry_chain = HOL.trans[OF diff_conv_add_uminus word_plus_carry_chain]
-
-lemma rev_bl_order_carry_chain:
-  "length xs = length ys \<Longrightarrow>
-    rev_bl_order F xs ys = (if xs = [] then F else
-        carry (\<not> (last (carry_chain (zip xs (map Not ys)) (\<not> F)))) (\<not> (last xs)) (last ys))"
-  apply (induct arbitrary: F rule: list_induct2)
-   apply (simp_all add: rev_bl_order_simps zip_eq_Nil_iff)
-  apply (intro impI conjI, simp_all)
-   apply (simp add: carry_def)
-   apply blast
-  apply (rule arg_cong[where f="\<lambda>x. carry x _ _"])
-  apply simp
-  apply (rule arg_cong[where f="last"])
-  apply (rule arg_cong[where f="carry_chain _"])
-  apply (simp add: carry_def)
-  apply blast
-  done
-
-lemma rev_bl_order_to_bl_carry_chain:
-  fixes x :: "('a :: len) word"
-  shows "rev_bl_order F (rev (to_bl x)) (rev (to_bl y)) =
-    carry (\<not> msb (carry_word x (NOT y) (\<not> F))) (\<not> msb x) (msb y)"
-  apply (simp add: rev_bl_order_carry_chain last_rev word_msb_alt)
-  apply (simp add: hd_rev[symmetric] zip_eq_Nil_iff Let_def)
-  apply (simp add: carry_word_def word_bl.Abs_inverse bl_word_not rev_map hd_map)
-  done
-
-(* the silly cw AND cw part is to stop the let_alt simproc removing the let-binding *)
-lemma word_le_carry_chain:
-  fixes x :: "('a :: len) word"
-  shows "(x \<le> y) = (let xnm = x; ynm = NOT y; cw = carry_word xnm ynm False in
-    carry (~ msb (cw AND cw)) (~ msb xnm) (~ msb ynm))"
-  by (simp add: word_le_rbl rev_bl_order_to_bl_carry_chain Let_def word_ops_msb)
-
-lemmas word_less_carry_chain = word_le_carry_chain[THEN arg_cong[where f=Not],
-    simplified linorder_not_le]
-
-lemma map_last_flip_to_xor:
-  fixes x :: "('a :: len) word"
-  shows "map_last Not (rev (to_bl x)) = rev (to_bl (x XOR (1 << (size x - 1))))"
-  apply (rule nth_equalityI, simp_all add: word_size map_last_def)
-  apply (simp add: nth_append nth_rev to_bl_nth nth_tl word_size word_ops_nth_size)
-  apply (simp add: nth_shiftl last_conv_nth rev_nth to_bl_nth flip: shiftl_1)
-  apply (intro conjI impI arg_cong2[where f="test_bit"], simp_all add: word_size)
-  done
-
-lemma word_sle_xor_eq_le[simplified word_size]:
-  "(x <=s y) = (x XOR (1 << (size x - 1)) \<le> y XOR (1 << (size x - 1)))"
-  by (simp add: word_sle_rbl word_le_rbl map_last_flip_to_xor word_size)
-
-lemma word_sless_xor_eq_le[simplified word_size]:
-  "(x <s y) = (x XOR (1 << (size x - 1)) < y XOR (1 << (size x - 1)))"
-  by (simp add: word_sless_rbl word_less_rbl map_last_flip_to_xor word_size)
-
 lemma minus_one_nat_case:
   "(n - 1) = (case n of 0 \<Rightarrow> 0 | Suc j \<Rightarrow> j)"
   by (simp split: nat.split)
-
-lemma carry_chain_nth:
-  "i < length xs \<Longrightarrow> nth (carry_chain xs F) i = (case i of 0 \<Rightarrow> F | Suc j \<Rightarrow>
-    carry (fst (nth xs j)) (snd (nth xs j)) (nth (carry_chain xs F) j))"
-proof (induct i arbitrary: F xs)
-  case 0
-  then show ?case
-    by (cases xs; simp)
-next
-  case (Suc i)
-  from Suc.prems show ?case
-    apply (cases xs; simp)
-    apply (simp add: Suc.hyps)
-    apply (simp split: nat.split)
-    done
-qed
-
-lemma carry_word_nth:
-  fixes x :: "('a :: len) word"
-  shows "i < LENGTH ('a) \<Longrightarrow>
-    test_bit (carry_word x y F) i = (case i of 0 \<Rightarrow> F | Suc j \<Rightarrow> carry (test_bit x j) (test_bit y j)
-        (test_bit (carry_word x y F) j))"
-  apply (simp add: carry_word_def test_bit_of_bl carry_chain_nth)
-  apply (simp add: test_bit_bl word_size carry_word_def split: nat.split)
-  apply (simp add: word_bl.Abs_inverse)
-  done
-
-lemma carry_word_eq_eq:
-  fixes x :: "('a :: len) word"
-  shows "(carry_word x y F = z) = (\<forall>i \<in> set (upt 0 (LENGTH ('a))).
-    (case i of 0 \<Rightarrow> F | Suc j \<Rightarrow> carry (test_bit x j) (test_bit y j) (test_bit z j)) = test_bit z i)"
-  apply (rule iffI)
-   apply (clarsimp simp: carry_word_nth)
-  apply (simp add: word_eq_iff Ball_def)
-  apply (rule allI, induct_tac n)
-   apply (intro impI, drule spec, drule(1) mp)
-   apply (simp add: carry_word_nth)
-  apply (intro impI, drule spec, drule(1) mp)
-  apply (simp add: carry_word_nth[where i="Suc _"])
-  done
 
 lemma upt_Suc_left:
   "upt (Suc i) j = (if j = 0 then [] else map Suc (upt i (j - 1)))"
   by (cases j, simp_all add: map_Suc_upt)
 
-lemma carry_word_eq_rbl:
-  fixes x :: "('a :: len) word"
-  shows "(carry_word x y F = z) = (F = test_bit z 0 \<and> (\<forall>(i, (xb, yb)) \<in> set (zip (upt 1 (LENGTH ('a)))
-        (zip (rev (to_bl x)) (rev (to_bl y)))).
-    carry xb yb (test_bit z (case i of 0 \<Rightarrow> 0 | Suc j \<Rightarrow> j)) = test_bit z i))"
-  apply (simp only: carry_word_eq_eq)
-  apply (subst upt_rec[where i=0])
-  apply (simp add: upt_Suc_left del: set_upt)
-  apply (simp add: all_set_conv_all_nth, simp add: Ball_def)
-  apply (intro conj_cong arg_cong[where f=All] ext imp_cong refl)
-  apply (frule order_less_le_trans[OF _ diff_le_self])
-  apply (simp add: test_bit_bl word_size)
-  done
+lemma upt_map_diff:
+  "upt i j = map ((+) i) (upt 0 (j - i))"
+  using map_add_upt[of i "j - i", symmetric]
+  by (cases "i \<le> j", simp_all)
 
 lemma word_if_add_let:
   "(if P then (x :: ('a :: len0) word) else y) = (let switch = P in id If switch x y)"
-  by simp
-
-lemma rbl_plus_simp_let:
-  "rbl_plus cin (x # xs) (y # ys) =
-    xor3 x y cin # (let c = carry x y cin in rbl_plus c xs ys)"
-  by (simp add: rbl_plus_def)
-
-lemma rev_bl_order_simp_let:
-  "rev_bl_order F (x # xs) (y # ys) =
-    (let xv = x; yv = y in rev_bl_order ((yv \<and> \<not> xv) \<or> ((yv \<or> \<not> xv) \<and> F)) xs ys)"
-  by (simp add: rev_bl_order_simps)
-
-lemma let_cons_expand:
-  "(let xs = b # bs in f xs) = (let hd_x = b; tl_xs = bs in f (hd_x # tl_xs))"
-  by simp
-
-lemma let_word_rbl:
-  "(let x = w in f x) = (let bs = rev (to_bl w) in f (of_bl (rev bs)))"
-  by simp
-
-lemma let_reassoc:
-  "(let x = (let y = vy in f y) in g x) = (let y = vy; x = f y in g x)"
-  by simp
-
-lemma rev_to_bl_of_bl[OF refl, simplified word_size]:
-  "w = of_bl xs \<Longrightarrow> rev (to_bl w) = takefill False (size w) (rev xs)"
-  by (simp add: word_rev_tf word_size)
-
-lemma lift_let:
-  "f (let x = v in g x) = (let x = v in f (g x))"
-  by simp
-
-lemmas lift_let_binop = lift_let[where f="\<lambda>x. f x y" for f y] lift_let[where f="f x" for f x]
-
-lemma takefill_last_empty_let:
-  "takefill_last z n [] = (let bit = z in replicate n bit)"
-  by (simp add: takefill_last_simps)
-
-lemmas takefill_last_simps2 = takefill_last_simps(1-2) takefill_last_empty_let
-
-lemma rbl_succ2_simp_let:
-  "rbl_succ2 b (x # xs) = (b \<noteq> x) # (let c = x \<and> b in rbl_succ2 c xs)"
-  by (simp_all add: rbl_succ2_def)
-
-lemmas rbl_succ2_simps2 = rbl_succ2_simps(1) rbl_succ2_simp_let
-
-lemmas bitwise_let_lifts =
-    lift_let[where f="case_prod f" for f]
-    lift_let[where f="case_list y f" for y f]
-    lift_let_binop[where f="(=)"]
-    lift_let[where f="map f" for f]
-    lift_let_binop[where f="zip"]
-    lift_let[where f="drop n" for n]
-    lift_let[where f="foldr f" for f]
-    lift_let[where f="takefill f n" for f n]
-    lift_let[where f="drop_nonempty v n" for v n]
-    lift_let_binop[where f="rev_bl_order f" for f]
-    lift_let_binop[where f="list_all2 f" for f]
-    lift_let[where f="rbl_succ2 x" for x]
-    lift_let_binop[where f="rbl_plus cin" for cin]
-    lift_let_binop[where f="append"]
-    lift_let[where f="takefill_last z n" for z n]
-
-lemmas logic_let_lifts =
-    lift_let_binop[where f="(\<longrightarrow>)"]
-    lift_let_binop[where f="(\<and>)"]
-    lift_let_binop[where f="(\<or>)"]
-    lift_let_binop[where f="(=)"]
-    lift_let[where f="Not"]
-
-lemmas imp_to_id = id_apply[where x="(\<longrightarrow>)", THEN fun_cong, THEN fun_cong, symmetric]
-
-lemma let_eqI:
-  "(\<And>x. v = x \<Longrightarrow> f x) \<Longrightarrow> let x = v in f x"
-  by simp
-
-lemma let_eq_impI:
-  "(\<And>x. v = x \<longrightarrow> P x) \<Longrightarrow> let x = v in P x"
   by simp
 
 ML \<open>
@@ -301,15 +59,16 @@ fun has_bv (Bound _) = true
   | has_bv (f $ x) = has_bv f orelse has_bv x
   | has_bv _ = false
 
-fun count_no_bv (t :: ts) tab = let
+fun count_no_bv pred (t :: ts) tab = let
     val ts = case t of
         f $ x => f :: x :: ts
       | Abs (_, _, t) => t :: ts
       | _ => ts
     val tab = if has_bv t then tab
-        else Termtab.map_default (t, 0) (fn i => i + 1) tab
-  in count_no_bv ts tab end
-  | count_no_bv [] tab = tab
+        else if pred t then Termtab.map_default (t, 0) (fn i => i + 1) tab
+        else tab
+  in count_no_bv pred ts tab end
+  | count_no_bv _ [] tab = tab
 
 val sym_def = @{thm Let_def[symmetric]}
 
@@ -318,12 +77,11 @@ fun add_let_conv ctxt nm x ct = let
   in Drule.infer_instantiate ctxt [(("f", 0), abs), (("s", 0), x)] sym_def end
 
 fun let_gather_dup_conv_1 ctxt f ct = let
-    val count = count_no_bv [Thm.term_of ct] Termtab.empty
+    val count = count_no_bv f [Thm.term_of ct] Termtab.empty
     val xs = Termtab.dest count
       |> filter (fn (_, j) => j >= 2)
       |> map fst
       |> filter (not o is_atom)
-      |> filter f
     fun get_greatest [] t _ = t
       | get_greatest (x :: xs) t sz = if size_of_term x > sz
         then get_greatest xs x (size_of_term x)
@@ -376,101 +134,135 @@ declare [[simproc del: let_alt]]
 simproc_setup let_atom ("Let v f") = \<open>K (K (Let_Alt.simproc false))\<close>
 declare [[simproc del: let_atom]]
 
+lemma let_eq_impI:
+  "(\<And>x. v = x \<Longrightarrow> P x) \<Longrightarrow> let x = v in P x"
+  by simp
+
+lemmas carry_let_eq_impI = let_eq_impI[where v="carry_val x y c", unfolded carry_val_word_eq_eq]
+  for x :: "('a :: len) word" and y c
+
+lemmas word_let_eq_impI = let_eq_impI[where v=x, unfolded word_bit_eq_iff]
+  for x :: "('a :: len) word"
+
+lemma case_nat_eq_If:
+  "(case n of 0 \<Rightarrow> x | Suc i \<Rightarrow> f i) = (if n = 0 then x else f (n - 1))"
+  by (cases n, auto)
+
+lemma ball_insert:
+  "(\<forall>x \<in> insert y S. P x) = (P y \<and> (\<forall>x \<in> S. P x))"
+  by simp
+
+lemmas imp_to_id = id_apply[where x="(\<longrightarrow>)", THEN fun_cong, THEN fun_cong, symmetric]
+
+ML \<open>
+structure Mk_Cache_Simproc = struct
+
+fun app cache ss ctxt ct = case Termtab.lookup (! cache) (Thm.term_of ct) of
+    SOME v => v
+  | NONE => let
+    val res = Simplifier.rewrite (put_simpset ss ctxt) ct
+    val res2 = if Thm.is_reflexive res then NONE else SOME res
+    val tab = Termtab.insert (K false) (Thm.term_of ct, res2) (! cache)
+  in cache := tab; res2 end
+
+fun mk ctxt nm ss lhss = Simplifier.make_simproc ctxt nm
+    {lhss = lhss, proc = K (app (Unsynchronized.ref Termtab.empty) ss)}
+
+end
+\<close>
+
 ML \<open>
 structure BW_Alt = struct
 
-open Word_Bitwise_Tac
+(* strategy:
+  1) rewrite with word_via_carry_val and word_if_add_let introducing lets
+  (init_tac)
+  2a) lift lets to top of goal and then to assumptions (let_eq_impI)
+    - also convert carry equals and other word equals to bitwise eqs
+  2b) pull assumptions with "bit" or "test_bit" back into the goal
+  (let_tac)
+  3a) hide implications from the simplifier (imp_to_id)
+      and unfold remaining word eqs to bitwise
+  3b) simplify with:
+    - caching simproc for natural arithmetic and word lengths
+    - upt/ball rules
+    - bit substitutions
+    - exp_eq_zero_iff from Word (2 ^ n = 0 \<longrightarrow> ineq)
+  3c) restore implications
+  (main_tac)
+*)
 
 val no_split_ss =
   simpset_of (put_simpset HOL_ss \<^context>
         delsimprocs [@{simproc let_simp}]
+        delsimps @{thms subst_all}
     |> Splitter.del_split @{thm if_split});
 
 val init_ss = simpset_of (put_simpset HOL_basic_ss \<^context> addsimps
-   @{thms word_eq_rbl_eq word_le_carry_chain word_less_carry_chain
-        word_sle_xor_eq_le word_sless_xor_eq_le})
+   @{thms word_via_carry_val word_if_add_let})
 
-val expand_word_eq_sss = map simpset_of [
-   put_simpset no_split_ss \<^context> addsimps
-    @{thms rbl_word_plus rbl_word_and rbl_word_or rbl_word_not
-                                rbl_word_neg bl_word_sub rbl_word_xor
-                                rbl_word_cat rbl_word_slice rbl_word_scast
-                                rbl_word_ucast rbl_shiftl rbl_shiftr rbl_sshiftr
-                                rbl_word_if_let lift_let[where f=to_bl]
-                                lift_let[where f=rev]
-                                rev_to_bl_of_bl rev_rev_ident},
-   put_simpset no_split_ss \<^context> addsimps
-    @{thms to_bl_numeral to_bl_neg_numeral to_bl_0 rbl_word_1},
-   put_simpset no_split_ss \<^context> addsimps
-    @{thms rev_rev_ident rev_replicate rev_map to_bl_upt word_size minus_one_nat_case}
-          addsimprocs [word_len_simproc],
-   put_simpset no_split_ss \<^context> addsimps
-    @{thms split_conv replicate.simps list.simps
-                                zip_Cons_Cons zip_Nil drop_Suc_Cons drop_0 drop_Nil
-                                foldr.simps zip.simps(1) takefill_Suc_Cons
-                                takefill_Suc_Nil takefill.Z rbl_succ2_simps2
-                                rbl_plus_simp_let rbl_plus_simps(2-)
-                                rev_bin_to_bl_simps append.simps
-                                takefill_last_simps2 drop_nonempty_simps
-                                rev_bl_order_simp_let rev_bl_order_simps(1)
-                                bitwise_let_lifts let_cons_expand
-                                ball_simps nat.simps
-                                let_reassoc[where f="_ :: _ \<Rightarrow> _ list" for f]
-                                Let_def[where f="\<lambda>_. []"]}
-          addsimprocs [expand_upt_simproc,
-                       @{simproc let_atom},
-                       nat_get_Suc_simproc 1
-                         [\<^term>\<open>replicate\<close>, \<^term>\<open>takefill x\<close>,
-                          \<^term>\<open>drop\<close>, \<^term>\<open>bin_to_bl\<close>,
-                          \<^term>\<open>takefill_last x\<close>,
-                          \<^term>\<open>drop_nonempty x\<close>,
-                          @{term \<open>nat.case_nat x y\<close>}]],
-    put_simpset no_split_ss \<^context> addsimps @{thms xor3_simps carry_simps if_bool_simps
-            Let_def[where s=True] Let_def[where s=False] One_nat_def id_apply}
-        addsimprocs [@{simproc let_alt}]
-  ]
+fun init_tac ctxt =
+    simp_tac (put_simpset init_ss ctxt addsimprocs [@{simproc let_alt}])
 
 val is_word = can Word_Lib.dest_wordT o fastype_of
 
-fun rev_mp_prems_tac pred ctxt = SUBGOAL (fn (t, i) => let
+fun rev_mp_prems_step_tac pred ctxt = DETERM o SUBGOAL (fn (t, i) => let
     val prems = Logic.strip_assums_hyp t
     val idx = find_index (fn t => can HOLogic.dest_Trueprop t andalso pred t) prems
   in
-    if idx = ~1 then all_tac
-    else EVERY' [rotate_tac idx, eresolve_tac ctxt @{thms rev_mp}, rotate_tac (~ idx),
-        rev_mp_prems_tac pred ctxt] i
+    if idx = ~1 then no_tac
+    else EVERY' [rotate_tac idx, eresolve_tac ctxt @{thms rev_mp}, rotate_tac (~ idx)] i
   end)
 
+fun rev_mp_prems_tac pred ctxt = REPEAT_DETERM o (rev_mp_prems_step_tac pred ctxt)
+
 fun let_to_imp_step ctxt = FIRST'
-  [resolve_tac ctxt @{thms let_eq_impI},
+  [resolve_tac ctxt @{thms carry_let_eq_impI word_let_eq_impI let_eq_impI},
    CHANGED o Let_Alt.let_to_top_tac ctxt,
    CHANGED o Let_Alt.let_gather_dup_tac ctxt is_word]
 
 fun let_to_imp_tac ctxt = TRY o REPEAT_ALL_NEW (let_to_imp_step ctxt)
 
-fun core_tacs ctxt = [
-    (CHANGED o safe_full_simp_tac (put_simpset init_ss ctxt addsimprocs [@{simproc let_alt}])),
-    rev_mp_prems_tac (exists_Const (fn (s, _) =>
-        s = @{const_name to_bl} orelse s = @{const_name carry_word})) ctxt,
-    safe_simp_tac (put_simpset HOL_basic_ss ctxt addsimps
-        @{thms word_plus_carry_chain word_minus_carry_chain word_if_add_let}),
-    let_to_imp_tac ctxt,
-    safe_simp_tac (put_simpset HOL_basic_ss ctxt addsimps
-        @{thms id_apply carry_word_eq_rbl msb_nth word_bw_same}),
-    safe_simp_tac (put_simpset HOL_basic_ss ctxt addsimps @{thms imp_to_id}),
-    safe_simp_tac (put_simpset init_ss ctxt)] @
-    map (fn ss => safe_simp_tac (put_simpset ss ctxt)) expand_word_eq_sss
+fun let_tac ctxt = let_to_imp_tac ctxt
+    THEN_ALL_NEW rev_mp_prems_tac (exists_Const (fn (s, _) => s = @{const_name bit})) ctxt
 
-fun core_tac ctxt = foldr1 (op THEN_ALL_NEW) (core_tacs ctxt)
+val len_ss = put_simpset (simpset_of \<^theory_context>\<open>Type_Length\<close>) @{context}
+        delsimps @{thms bit_0}
+    |> simpset_of;
 
-fun expand_tac ctxt = core_tac ctxt
-    THEN_ALL_NEW safe_full_simp_tac
-        (put_simpset no_split_ss ctxt addsimps @{thms Let_def})
+fun mk_arith_simproc ctxt = Mk_Cache_Simproc.mk ctxt "bitwise_arith_cache" len_ss
+  (map Logic.varify_global
+    [@{term "x + y"}, @{term "x - y"}, @{term "Suc i"}, @{term "x < y"},
+        @{term "x = y"}, @{term "x <= y"},
+        @{term "len_of x"}])
 
-fun lift_tac ctxt = core_tac ctxt
-    THEN_ALL_NEW simp_tac
-        (put_simpset HOL_basic_ss ctxt addsimps @{thms logic_let_lifts})
-    THEN_ALL_NEW (TRY o DETERM o REPEAT_ALL_NEW (resolve_tac ctxt @{thms let_eqI}))
+fun get_bit_simps ctxt = Named_Theorems.get ctxt @{named_theorems bit_simps}
+
+fun main_ss ctxt = put_simpset no_split_ss ctxt
+    addsimps @{thms Word.exp_eq_zero_iff
+        upt_conv_Cons numeral_2_eq_2[symmetric]
+        upt_conv_Nil[OF order_refl]
+        list.set ball_insert ball_empty}
+    addsimps (get_bit_simps ctxt)
+    addsimprocs [mk_arith_simproc ctxt]
+
+fun main_tac ctxt =
+    simp_tac (put_simpset HOL_basic_ss ctxt addsimps @{thms imp_to_id word_bit_eq_iff})
+    THEN_ALL_NEW simp_tac (main_ss ctxt)
+    THEN_ALL_NEW simp_tac (put_simpset HOL_basic_ss ctxt addsimps @{thms id_apply simp_thms})
+
+fun tac ctxt = init_tac ctxt
+    THEN_ALL_NEW let_tac ctxt
+    THEN_ALL_NEW main_tac ctxt
+
+(* also pull in assumptions that can be rewritten bitwise *)
+
+fun asm ctxt = full_simp_tac (put_simpset HOL_basic_ss ctxt
+        addsimps @{thms word_ineq_via_carry_val word_bit_eq_iff})
+    THEN_ALL_NEW rev_mp_prems_tac (exists_Const (fn (s, _) => s = @{const_name bit}
+        orelse s = @{const_name carry_val})) ctxt
+
+fun asm_tac ctxt = asm ctxt THEN_ALL_NEW tac ctxt
 
 end
 \<close>
@@ -479,19 +271,36 @@ method_setup let_dup_word =
   \<open>Scan.succeed (fn ctxt => Method.SIMPLE_METHOD (Let_Alt.let_gather_dup_tac ctxt BW_Alt.is_word 1))\<close>
   "gather repeated word terms using let-binding"
 
-method_setup word_bitwise =
-  \<open>Scan.succeed (fn ctxt => Method.SIMPLE_METHOD (BW_Alt.expand_tac ctxt 1))\<close>
-  "decomposer for word equalities and inequalities into bit propositions"
-
 method_setup word_bitwise_eq =
-  \<open>Scan.succeed (fn ctxt => Method.SIMPLE_METHOD (BW_Alt.lift_tac ctxt 1))\<close>
+  \<open>Scan.succeed (fn ctxt => Method.SIMPLE_METHOD (BW_Alt.tac ctxt 1))\<close>
   "decomposer for word equalities and inequalities into bit propositions,
     lifting shared booleans to variables"
 
+lemma (* testing *)
+  fixes x :: "8 word" and y :: "6 word"
+  shows "or (and (ucast x) (xor y 0)) (xor y 0) = y"
+  apply (tactic \<open>BW_Alt.init_tac @{context} 1\<close>)
+  apply (tactic \<open>BW_Alt.let_tac @{context} 1\<close>)
+  apply (tactic \<open>BW_Alt.main_tac @{context} 1\<close>)
+  apply blast
+  done
+
+lemma (* testing *)
+  fixes x :: "8 word" and y :: "6 word"
+  shows "or (and (ucast x) (xor y 0)) (xor y 0) = y"
+  apply word_bitwise_eq
+  apply blast
+  done
+
+end
+
+
 lemma test_bit_is_slice_check:
   fixes x :: "('a :: len) word"
-  shows "test_bit x n = (Word.slice n x = (1 :: 1 word))"
-  by (simp add: word_eq_iff nth_slice)
+  shows "bit x n = (Word.slice n x = (1 :: 1 word))"
+  unfolding word_bit_eq_iff
+  using bit_imp_le_length[of x n]
+  by (auto simp add: bit_simps simp flip: bit_0)
 
 lemma word_set_bit_to_smt:
   fixes x :: "('a :: len0) word"
